Added failing test

Source/DafnyCore.Test/GeneratedDafnyTest.cs
@@ -6,7 +6,12 @@ namespace DafnyCore.Test;
 public class GeneratedDafnyTest {
   [Fact]
   public void TestDafnyCoverage() {
-    DafnyToRustCompilerCoverage.RASTCoverage.__default.TestExpr();
+    DafnyToRustCompilerCoverage.__default.TestIsCopy();;
+  }
+  
+  [Fact]
+  public void TestRustASTCoverage() {
+    RASTCoverage.__default.TestExpr();
   }
 
   [Fact]
